### The Electric Field Due to a Charged Disk
- The last section was about *linear* charge densities
    * This one will use the same methodology with **surface charge density($\sigma$)**
        + DON'T FREAK OUT; we don't have to go through that whole procedure again


#### The Problem
- Imagine a circular disk of radius R and uniform charge $q$ described by $\sigma$ and a point P along the central axis
    * Now, superimpose a ring of radius $r$ and charge $dq$
        + *Do you see where this is going?*
    * We know that the $\vec{E}$ exerted on P by the differential ring is
$$ \vec{E} = \frac{z q_{total}}{4 \pi \epsilon_0 \big( R^2 + z^2 \big)^\frac{3}{2}} $$
- Making the appropriate substitutions, we get

$$ d\vec{E} = \frac{z dq}{4 \pi \epsilon_0 \big( r^2 + z^2 \big)^\frac{3}{2}} $$
- Now, we just have to define $dq$ in terms of our integrating variable, $r$
- Consider the following
$$ dq = \sigma (2 \pi r) dr $$
- This just indicates that our differential charge along each ring is equal to the surface charge density multiplied by the differential area that ring occupies
- Making that substitution,
$$ d\vec{E} = \frac{z \sigma (2 \pi r) dr }{4 \pi \epsilon_0 \big( r^2 + z^2 \big)^\frac{3}{2}} $$
$$ d\vec{E} = \bigg[ \frac{z \sigma (2 \pi r) }{4 \pi \epsilon_0 \big( r^2 + z^2 \big)^\frac{3}{2}} \bigg] dr $$
$$ d\vec{E} = \bigg[ \frac{z \sigma r }{2 \epsilon_0 \big( r^2 + z^2 \big)^\frac{3}{2}} \bigg] dr $$
- Now, we integrate both sides
$$ \int_{r=0}^{r=R} d\vec{E} = \int_{r=0}^{r=R} \bigg[ \frac{z \sigma r }{2 \epsilon_0 \big( r^2 + z^2 \big)^\frac{3}{2}} \bigg] dr $$
- Much of the integrand is composed of constants, which we can factor out
$$ \int_{r=0}^{r=R} d\vec{E} = \frac{z \sigma}{2 \epsilon_0} \int_{r=0}^{r=R} \bigg[ \frac{r}{\big( r^2 + z^2 \big)^\frac{3}{2}} \bigg] dr $$
$$ \vec{E} = \frac{z \sigma}{2 \epsilon_0} \int_{r=0}^{r=R} \bigg[ \frac{r}{\big( r^2 + z^2 \big)^\frac{3}{2}} \bigg] dr $$
- We can solve this integral by using u-substitution
$$ u = \big( r^2 + z^2 \big) $$
$$ \frac{du}{dr} = \frac{1}{dr} \bigg[ \big( r^2 + z^2 \big) \bigg]$$
$$ \frac{du}{dr} = \big( 2 r \big) $$
$$ du = \big( 2 r \big) dr $$
$$ dr = \frac{1}{\big( 2 r \big)} du $$
- We can convert our limits of integration from r units to u units by
$$ u = \big( r^2 + z^2 \big) $$
- Making that substitution, our integral becomes
$$ \vec{E} = \frac{z \sigma}{2 \epsilon_0} \int_{u=z^2}^{u=R^2 + z^2} \bigg( \frac{r}{u^\frac{3}{2}} \bigg) (\frac{1}{2 r} du) $$
$$ \vec{E} = \frac{z \sigma}{4 \epsilon_0} \int_{u=z^2}^{u=R^2 + z^2} \bigg( \frac{1}{u^\frac{3}{2}} \bigg) du $$
$$ \vec{E} = \frac{z \sigma}{4 \epsilon_0} \int_{u=z^2}^{u=R^2 + z^2} \bigg( u^{ - \frac{3}{2}} \bigg) du $$
$$ \vec{E} = \frac{z \sigma}{4 \epsilon_0} \bigg[ \frac{u^{- \frac{1}{2}}}{- \frac{1}{2}} \bigg]_{z^2}^{R^2 + z^2} $$
$$ \vec{E} = \frac{z \sigma}{4 \epsilon_0} \bigg[ \frac{-2}{\sqrt{u}} \bigg]_{u=z^2}^{u=R^2 + z^2} $$
$$ \vec{E} = - \frac{z \sigma}{2 \epsilon_0} \bigg[ \frac{1}{\sqrt{u}} \bigg]_{u=z^2}^{u=R^2 + z^2} $$
$$ \vec{E} = - \frac{z \sigma}{2 \epsilon_0} \bigg[ \frac{1}{\sqrt{R^2 + z^2}} - \frac{1}{\sqrt{z^2}} \bigg] $$
$$ \vec{E} = \frac{z \sigma}{2 \epsilon_0} \bigg[ \frac{1}{\sqrt{z^2}} - \frac{1}{\sqrt{R^2 + z^2}} \bigg] $$
$$ \vec{E} = \frac{z \sigma}{2 \epsilon_0} \bigg[ \frac{1}{z} - \frac{1}{\sqrt{R^2 + z^2}} \bigg] $$
$$ \vec{E} = \frac{\sigma}{2 \epsilon_0} \bigg[ \frac{z}{z} - \frac{z}{\sqrt{R^2 + z^2}} \bigg] $$
$$ \vec{E} = \frac{\sigma}{2 \epsilon_0} \bigg[ 1 - \frac{z}{\sqrt{R^2 + z^2}} \bigg] $$
- And thus, the problem is solved.  Isn't calculus fun?
